src/lib/kuiper/Kuiper.Real.fst
@@ -87,6 +87,14 @@ let rsum_append (s1 s2 : Seq.seq real)
       seq_fold_left (+.) 0.0R s1 +. seq_fold_left (+.) 0.0R s2;
     }
 
+let lem_rmax_comm (x: real) (y: real)
+  : Lemma (ensures rmax x y == rmax y x)
+  = ()
+
+let lem_rmax_assoc (x: real) (y: real) (z: real)
+  : Lemma (ensures rmax x (rmax y z) == rmax (rmax x y) z)
+  = ()
+
 let rec sum_non_zero
     (s : Seq.seq real { forall (i:natlt (Seq.length s)). Seq.index s i >. 0.0R })
     (acc : real)
